improved notations

src/Refinement.v
@@ -10,56 +10,8 @@ From MRC Require Import Stdppp.
 From MRC Require Import PredCalc.
 From MRC Require Import Prog.
 
-(*TODO: move it, probably the non-prime one is useless *)
-Instance feval_proper_fent' {M σ} : Proper ((@fent M) ==> impl) (feval σ).
-Proof.
-  intros A B H H0. apply H. apply H0.
-Qed.
-
-Definition of_same_length_eq_l {A B} {l1 l1' : list A} {l2 : list B} (H : OfSameLength l1 l2) :
-  l1 = l1' →
-  OfSameLength l1' l2.
-Proof. intros. subst. exact H. Qed.
-
-Definition of_same_length_eq_r {A B} {l1 : list A} {l2 l2' : list B} (H : OfSameLength l1 l2) :
-  l2 = l2' →
-  OfSameLength l1 l2'.
-Proof. intros. subst. exact H. Qed.
-
-Definition of_same_length_eq {A B} {l1 l1' : list A} {l2 l2' : list B} (H : OfSameLength l1 l2) :
-  l1 = l1' →
-  l2 = l2' →
-  OfSameLength l1' l2'.
-Proof. intros. subst. exact H. Qed.
-
 Open Scope stdpp_scope.
 Open Scope refiney_scope.
-
-(* TODO: move it *)
-#[global] Hint Unfold universal_relation : core.
-(* Lemma lookup_list_to_map_zip_cons_ne {K A} `{Countable K} *)
-(*     (ks : list K) (xs : list A) (k : K) (x : A) (i : K) `{OfSameLength K A ks xs} : *)
-(*   k ≠ i → *)
-(*   (list_to_map (zip (k :: ks) (x ::xs)) : gmap K A) !! i = *)
-(*     (list_to_map (zip ks xs) : gmap K A) !! i. *)
-(* Proof with auto. *)
-(*   intros. simpl. rewrite lookup_insert_ne... *)
-(* Qed. *)
-(* Proof with auto. *)
-(*   remember (length ks) as n eqn:E. symmetry in E. generalize dependent xs. *)
-(*   generalize dependent ks. induction n; intros. *)
-(*   - simpl. apply length_zero_iff_nil in E. subst. simpl in H1. rewrite lookup_empty in H1. *)
-(*     discriminate. *)
-(*   - assert (E1:=E). rewrite of_same_length in E1. *)
-(*     apply length_nonzero_iff_cons in E as (k'&ks'&->&?). *)
-(*     apply length_nonzero_iff_cons in E1 as (x'&xs'&->&?). subst. simpl in H1. *)
-(*     destruct (decide (k' = k)). *)
-(*     + subst. rewrite lookup_insert in H1. exists 0. simpl. split... *)
-(*     + forward (IHn ks') by reflexivity. forward (IHn xs'). *)
-(*       { unfold OfSameLength... } *)
-(*       rewrite lookup_insert_ne in H1... destruct (IHn H1) as (i&?&?). *)
-(*       exists (S i). simpl. split... *)
-(* Qed. *)
 
 Section refinement.
   Context {M : model}.
@@ -71,8 +23,7 @@ Section refinement.
 
   Implicit Types A B C : formula.
   Implicit Types pre post : formula.
-  Implicit Types w : list final_variable.
-  Implicit Types xs : list final_variable.
+  Implicit Types w xs : list final_variable.
   (* Implicit Types ts : list term. *)
 
 
@@ -90,339 +41,15 @@ Section refinement.
     intros Hent A Hinit. simpl. f_simpl. assumption.
   Qed.
 
-  (* TODO: move it *)
-  Lemma teval_delete_bottom_state_var σ x t v :
-    x ∉ dom σ →
-    teval (<[x:=value_bottom M]> σ) t v ↔ teval σ t v.
-  Proof with auto.
-    intros. generalize dependent v. induction t; intros.
-    - split; inversion 1...
-    - split; inversion 1; subst x1.
-      + destruct (decide (x = x0)).
-        * subst x0. rewrite (lookup_total_insert σ) in H2. subst v0. constructor.
-          rewrite (lookup_total_alt σ). apply (not_elem_of_dom σ) in H. rewrite H.
-          simpl...
-        * rewrite (lookup_total_insert_ne σ) in H2...
-      + destruct (decide (x = x0)).
-        * subst x0 v0. rewrite (lookup_total_alt σ) in H2. apply (not_elem_of_dom σ) in H.
-          rewrite H in H2. simpl in H2. rewrite H2. constructor.
-          rewrite (lookup_total_insert σ)...
-        * constructor. rewrite (lookup_total_insert_ne σ)...
-    - split; inversion 1; subst; apply TEval_App with (vargs:=vargs)...
-      + clear H1 H6. generalize dependent vargs. induction args; intros.
-        * inversion H4. subst. constructor.
-        * inversion H4. subst. constructor.
-          -- rewrite <- H0... left...
-          -- apply IHargs... intros. apply H0. right...
-      + clear H1 H6. generalize dependent vargs. induction args; intros.
-        * inversion H4. subst. constructor.
-        * inversion H4. subst. constructor.
-          -- rewrite H0... left...
-          -- apply IHargs... intros. apply H0. right...
-  Qed.
-
-  Lemma afeval_delete_bottom_state_var σ x af :
-    x ∉ dom σ →
-    afeval (<[x:=value_bottom M]> σ) af ↔ afeval σ af.
-  Proof with auto.
-    intros. destruct af...
-    - simpl. setoid_rewrite teval_delete_bottom_state_var...
-    - simpl. split; intros (vargs&?&?); exists vargs; split; auto; clear H1;
-        generalize dependent vargs; induction args; intros; inversion H0; subst;
-        try constructor...
-      + rewrite <- (teval_delete_bottom_state_var _ x a v)...
-      + rewrite (teval_delete_bottom_state_var _ x a v)...
-  Qed.
-
-  Lemma feval_delete_bottom_state_var σ x A :
-    x ∉ dom σ →
-    feval (<[x:=value_bottom M]> σ) A ↔ feval σ A.
-  Proof with auto.
-    intros. induction A; simp feval.
-    2-5: naive_solver.
-    apply afeval_delete_bottom_state_var...
-  Qed.
-
-  Lemma f_exists_introduce_binder x A :
-    A ⇛ <! ∃ x, A !>.
-  Proof with auto.
-    intros σ H. simp feval. pose proof (teval_total σ x) as [v Hv].
-    exists v. rewrite feval_subst with (v:=v)... inversion Hv.
-    subst x0. subst v0. unfold state in *.
-    rewrite lookup_total_alt in H1. destruct (σ !! x) eqn:E.
-    + simpl in H1. subst. rewrite insert_id...
-    + simpl in H1. rewrite <- H1. rewrite feval_delete_bottom_state_var...
-      apply (not_elem_of_dom σ)...
-  Qed.
-
-  Lemma f_forall_drop_binder A x :
-    <! ∀ x, A !> ⇛ A.
-  Proof with auto.
-    unfold FForall. apply f_ent_contrapositive. rewrite f_not_stable.
-    apply f_exists_introduce_binder.
-  Qed.
-
-  (* Definition x := raw_var "x". *)
-  (* Definition y := raw_var "y". *)
-  (* Definition n2 := raw_var "2". *)
-  (* Definition n5 := raw_var "5". *)
-
-  (* Definition FSForall xs A := <! ∀* xs, A[[*xs \ ]] *)
-
-  (* Infix "⇛ₗ@{ M }" := (@fent M _) (at level 70, only parsing, no associativity) *)
-  (*     : refiney_scope. *)
-  (* Lemma play : *)
-  (*   @fent M *)
-  (*   <! ∀* $([y; x]), ⌜x = y + n2⌝ !> <! ⌜y = n5 + n2⌝ !>. *)
-  (* Proof. *)
-  (*   simpl. rewrite f_forall_elim with (t:=n5). *)
-  (*   rewrite f_forall_elim with (t:=y). *)
-  (*   rewrite simpl_subst_af. simpl. rewrite simpl_subst_af. simpl. *)
-  (*   simpl. *)
-  (*   unfold formula_subst. *)
-  (*   cbn. unfold quant_subst_skip_cond. *)
-  (*   simpl. *)
-  (*   simpl. hnf. *)
-  Lemma teval_var_term_map_det {σ} m mv mv' :
-    @teval_var_term_map M σ m mv →
-    @teval_var_term_map M σ m mv' →
-    mv = mv'.
-  Proof with auto.
-    intros. generalize dependent m. generalize dependent mv'.
-    induction mv as [| x v mv Hx IH] using map_ind; intros.
-    - destruct H as []. destruct H0 as []. rewrite <- H in H0. rewrite dom_empty_L in H0.
-      apply dom_empty_inv_L in H0. subst...
-    - assert (Hmv:=H). assert (Hmv':=H0). destruct H as []. destruct H0 as [].
-      rewrite dom_insert_L in H. symmetry in H. rewrite H in H0.
-      apply dom_union_inv_L in H as (m1&m2&?&?&?&?).
-      2: { apply disjoint_singleton_l. apply not_elem_of_dom... }
-      apply dom_singleton_inv_L in H4 as [t Ht]. subst m1.
-      rewrite <- insert_union_singleton_l in H. subst m. rename m2 into m.
-      apply dom_union_inv_L in H0 as (m1&m2&?&?&?&?).
-      2: { apply disjoint_singleton_l. apply not_elem_of_dom... }
-      apply dom_singleton_inv_L in H4 as [v' Hv']. subst m1.
-      rewrite <- insert_union_singleton_l in H. subst mv'. rename m2 into mv'.
-      assert (teval σ t v).
-      { apply H1 with (x:=x); apply lookup_insert... }
-      assert (teval σ t v').
-      { apply H2 with (x:=x); apply lookup_insert... }
-      clear H1 H2. pose proof (teval_det _ _ _ H H4) as ->. clear H H4.
-      apply (teval_var_term_map_delete x) in Hmv, Hmv'.
-      apply map_disjoint_singleton_l in H3, H0. rewrite (delete_insert) in Hmv, Hmv'...
-      rewrite (delete_insert) in Hmv, Hmv'... rewrite (IH mv' m)...
-  Qed.
-
-  Lemma teval_var_term_map_zip_cons_inv σ x (xs : list variable) t ts mv `{OfSameLength _ _ xs ts} :
-    NoDup (x :: xs) →
-    @teval_var_term_map M σ (to_var_term_map (x :: xs) (t :: ts)) mv →
-    ∃ v mv', teval σ t v ∧ mv = {[x := v]} ∪ mv' ∧ x ∉ dom mv'
-             ∧ @teval_var_term_map M σ (to_var_term_map xs ts) mv'.
-  Proof with auto.
-    intros. generalize dependent mv. generalize dependent ts. generalize dependent t.
-    generalize dependent x. induction xs as [|x' xs' IH]; intros; assert (Hl:=H).
-    - apply of_same_length_nil_inv_l in Hl as ->. unfold to_var_term_map in H1. simpl in H1.
-      destruct H1 as []. rewrite insert_empty in H1. rewrite dom_singleton_L in H1.
-      apply dom_singleton_inv_L in H1 as [v ->]. exists v, ∅. split_and!.
-      + eapply H2; [apply lookup_insert|apply lookup_singleton].
-      + rewrite map_union_empty...
-      + apply not_elem_of_empty.
-      + hnf. cbn. split... intros. apply lookup_empty_Some in H1 as [].
-    - apply of_same_length_cons_inv_l in Hl as (t'&ts'&->&?).
-      apply NoDup_cons in H0 as []. forward (IH x')...
-      apply of_same_length_rest in H as Hl. specialize (IH t' ts' Hl).
-      destruct H1 as []. unfold to_var_term_map in H1. rewrite dom_list_to_map_zip_L in H1.
-      2:{ typeclasses eauto. } rewrite list_to_set_cons in H1.
-      apply dom_union_inv_L in H1 as (m1&m2&?&?&?&?).
-      2: { set_solver. }
-      apply dom_singleton_inv_L in H6 as [v Hv]. subst m1.
-      rewrite <- insert_union_singleton_l in H1. subst mv. rename m2 into mv.
-      assert (teval_var_term_map σ (to_var_term_map (x' :: xs') (t' :: ts')) mv).
-      { split.
-        - unfold to_var_term_map. rewrite dom_list_to_map_zip_L...
-        - intros. assert (x0 ≠ x).
-          { intros contra. subst. apply elem_of_dom_2 in H6. rewrite H7 in H6.
-            apply elem_of_list_to_set in H6. contradiction. }
-          apply (H4 x0)...
-          ++ unfold to_var_term_map. simpl. rewrite lookup_insert_ne...
-          ++ rewrite lookup_insert_ne...
-      }
-      destruct (IH mv) as (v'&mv'&?&?&?&?)...
-      exists v, mv. split_and!...
-      + apply (H4 x).
-          * unfold to_var_term_map. simpl. rewrite lookup_insert...
-          * rewrite lookup_insert...
-        + rewrite insert_union_singleton_l...
-        + set_solver.
-  Qed.
-
-  Lemma f_existslist_as_foralllist (xs : list variable) A :
-    <! ∃* xs, A !> ≡ <! ¬ ∀* xs, ¬ A !>.
-  Proof with auto.
-    induction xs as [|x xs IH]; simpl...
-    - rewrite f_not_stable...
-    - intros σ. unfold FForall. rewrite IH... rewrite f_not_stable...
-  Qed.
-  (* Lemma f_exists_intro_as_ssubst A (xs : list variable) ts `{OfSameLength _ _ xs ts} : *)
-  (*   length xs ≠ 0 → *)
-  (*   NoDup xs → *)
-  (*   <! A[[*xs \ *ts]] !> ⇛ <! ∃* xs, A !>. *)
-  (* Proof with auto. *)
-  (*   generalize dependent ts. generalize dependent A. *)
-  (*   induction xs as [|x xs IH]; intros; assert (Hl:=H). *)
-  (*   1: { simpl in H0. contradiction. } *)
-  (*   apply of_same_length_cons_inv_l in Hl as (t&ts'&->&?). rename ts' into ts. *)
-  (*   clear H0. destruct (length xs) eqn:E. *)
-  (*   1:{ apply length_zero_iff_nil in E, H2. subst. simpl in *. rewrite (ssubst_single A x t). *)
-  (*       apply f_exists_intro... } *)
-  (*   apply of_same_length_rest in H as ?. clear E. simpl. assert (Hunique:=H1). *)
-  (*   apply NoDup_cons in H1 as []. rewrite f_exists_existslist_comm. *)
-  (*   intros σ ?. pose proof (teval_total σ t) as [vt Hvt]. *)
-  (*   rewrite f_exists_intro with (t:=TConst vt). *)
-  (*   specialize (IH <! A[x \ $(TConst vt)] !> ts H0). forward IH by lia. *)
-  (*   rewrite IH in H4... rewrite <- ssubst_extract_inside in H4... *)
-  (*   2: { simpl. set_solver. } *)
-  (*   pose proof (teval_var_term_map_total σ (to_var_term_map (x::xs) (t::ts))) as (mv&?). *)
-  (*   rewrite feval_simult_subst with (mv:=mv)... *)
-  (*   pose proof (teval_var_term_map_total σ (to_var_term_map (x::xs) ((TConst vt)::ts))) as (mv'&?). *)
-  (*   rewrite feval_simult_subst with (mv:=mv') in H4... *)
-  (*   enough (mv = mv') by (subst mv'; assumption). clear H2 IH H4 A. *)
-  (*   apply of_same_length_rest in H as Hl. *)
-  (*   apply teval_var_term_map_zip_cons_inv with (H:=Hl) in H5 as (v&mv0&?&->&?&?)... *)
-  (*   apply teval_var_term_map_zip_cons_inv with (H:=Hl) in H6 as (v'&mv1&?&->&?&?)... *)
-  (*   inversion H6. subst v0. subst v'. pose proof (teval_det t vt v Hvt H2) as ->. *)
-  (*   pose proof (teval_var_term_map_det _ _ _ H5 H8) as ->... *)
-  (* Qed. *)
-  Lemma f_foralllist_elim_as_ssubst A (xs : list variable) ts `{OfSameLength _ _ xs ts} :
-    length xs ≠ 0 →
-    NoDup xs →
-    <! ∀* xs, A !> ⇛ <! A[[*xs \ *ts]] !>.
-  Proof with auto.
-    generalize dependent ts. generalize dependent A.
-    induction xs as [|x xs IH]; intros; assert (Hl:=H).
-    1: { simpl in H0. contradiction. }
-    apply of_same_length_cons_inv_l in Hl as (t&ts'&->&?). rename ts' into ts.
-    clear H0. destruct (length xs) eqn:E.
-    1:{ apply length_zero_iff_nil in E, H2. subst. simpl in H1. rewrite (ssubst_single A x t).
-        apply f_forall_elim... }
-    apply of_same_length_rest in H as ?. clear E. simpl. assert (Hunique:=H1).
-    apply NoDup_cons in H1 as []. rewrite f_forall_foralllist_comm.
-    intros σ ?. pose proof (teval_total σ t) as [vt Hvt].
-    rewrite f_forall_elim with (t:=TConst vt) in H4.
-    specialize (IH <! A[x \ $(TConst vt)] !> ts H0). forward IH by lia.
-    rewrite IH in H4... rewrite <- ssubst_extract_inside in H4...
-    2: { simpl. set_solver. }
-    pose proof (teval_var_term_map_total σ (to_var_term_map (x::xs) (t::ts))) as (mv&?).
-    rewrite feval_simult_subst with (mv:=mv)...
-    pose proof (teval_var_term_map_total σ (to_var_term_map (x::xs) ((TConst vt)::ts))) as (mv'&?).
-    rewrite feval_simult_subst with (mv:=mv') in H4...
-    enough (mv = mv') by (subst mv'; assumption). clear H2 IH H4 A.
-    apply of_same_length_rest in H as Hl.
-    apply teval_var_term_map_zip_cons_inv with (H:=Hl) in H5 as (v&mv0&?&->&?&?)...
-    apply teval_var_term_map_zip_cons_inv with (H:=Hl) in H6 as (v'&mv1&?&->&?&?)...
-    inversion H6. subst v0. subst v'. pose proof (teval_det t vt v Hvt H2) as ->.
-    pose proof (teval_var_term_map_det _ _ _ H5 H8) as ->...
-  Qed.
-
-  Lemma simpl_ssubst_not A (xs : list variable) ts `{OfSameLength _ _ xs ts} :
-    <! (¬ A) [[*xs \ *ts]] !> ≡ <! ¬ (A [[*xs \ *ts]]) !>.
-  Proof. simp simult_subst. reflexivity. Qed.
-  Lemma simpl_ssubst_and A B (xs : list variable) ts `{OfSameLength _ _ xs ts} :
-    <! (A ∧ B) [[*xs \ *ts]] !> ≡ <! A [[*xs \ *ts]] ∧ B [[*xs \ *ts]] !>.
-  Proof. simp simult_subst. reflexivity. Qed.
-  Lemma simpl_ssubst_or A B (xs : list variable) ts `{OfSameLength _ _ xs ts} :
-    <! (A ∨ B) [[*xs \ *ts]] !> ≡ <! A [[*xs \ *ts]] ∨ B [[*xs \ *ts]] !>.
-  Proof. simp simult_subst. reflexivity. Qed.
-  Lemma simpl_ssubst_impl A B (xs : list variable) ts `{OfSameLength _ _ xs ts} :
-    <! (A ⇒ B) [[*xs \ *ts]] !> ≡ <! A [[*xs \ *ts]] ⇒ B [[*xs \ *ts]] !>.
-  Proof. unfold FImpl. simp simult_subst. reflexivity. Qed.
-  Lemma simpl_ssubst_iff A B (xs : list variable) ts `{OfSameLength _ _ xs ts} :
-    <! (A ⇔ B) [[*xs \ *ts]] !> ≡ <! A [[*xs \ *ts]] ⇔ B [[*xs \ *ts]] !>.
-  Proof. unfold FIff, FImpl. simp simult_subst. reflexivity. Qed.
-
-  Lemma f_exists_intro_as_ssubst A (xs : list variable) ts `{OfSameLength _ _ xs ts} :
-    length xs ≠ 0 →
-    NoDup xs →
-    <! A[[*xs \ *ts]] !> ⇛ <! ∃* xs, A !>.
-  Proof with auto.
-    intros. rewrite f_existslist_as_foralllist. rewrite <- f_ent_contrapositive.
-    rewrite f_not_stable. rewrite <- simpl_ssubst_not. apply f_foralllist_elim_as_ssubst...
-  Qed.
-
-  Lemma initial_free_in_final_formula x A :
-    formula_final A →
-    initial_var_of x ∉ formula_fvars A.
-  Proof.
-    intros. intros contra. apply H in contra. cbv in contra. discriminate.
-  Qed.
-
   Lemma r_contract_frame (x : final_variable) pre post `{FormulaFinal _ pre} :
     <{ x : [pre, post] }> ⊑ <{ : [pre, post[₀x\x] ] }>.
   Proof with auto.
-    intros A Hfree. simpl. f_simpl. rewrite f_forall_drop_binder.
+    intros A Hfree. simpl. f_simpl. rewrite f_forall_elim_binder.
     unfold subst_initials. simpl. rewrite simpl_subst_impl.
     rewrite fequiv_subst_non_free with (A:=A).
     - reflexivity.
-    - apply initial_free_in_final_formula...
+    - intros contra. apply initial_var_of_elem_of_formula_fvars in contra. contradiction.
   Qed.
-
-  Lemma f_existslist_app (xs1 xs2 : list variable) A :
-    <! ∃* $(xs1 ++ xs2), A !> ≡ <! ∃* xs1, ∃* xs2, A !>.
-  Proof with auto.
-    induction xs1 as [|x1 xs1 IH]... simpl. rewrite IH...
-  Qed.
-
-  Lemma f_foralllist_app (xs1 xs2 : list variable) A :
-    <! ∀* $(xs1 ++ xs2), A !> ≡ <! ∀* xs1, ∀* xs2, A !>.
-  Proof with auto.
-    induction xs1 as [|x1 xs1 IH]... simpl. rewrite IH...
-  Qed.
-
-  Lemma f_foralllist_drop_binders (xs : list variable) A :
-    <! ∀* xs, A !> ⇛ <! A !>.
-  Proof with auto.
-    induction xs as [|x xs IH]; simpl.
-    - reflexivity.
-    - rewrite IH. rewrite f_forall_drop_binder. reflexivity.
-  Qed.
-
-  Lemma f_existslist_introduce_binders (xs : list variable) A :
-    <! A !> ⇛ <! ∃* xs, A !>.
-  Proof with auto.
-    rewrite f_existslist_as_foralllist. rewrite <- f_ent_contrapositive. rewrite f_not_stable.
-    apply f_foralllist_drop_binders.
-  Qed.
-
-  Lemma f_eqlist_app ts1 ts1' ts2 ts2'
-                          `{OfSameLength _ _ (ts1 ++ ts1') (ts2 ++ ts2')}
-                          `{OfSameLength _ _ ts1 ts2}
-                          `{OfSameLength _ _ ts1' ts2'} :
-    <! ⌜$(ts1 ++ ts1') =* $(ts2 ++ ts2')⌝ !> ≡@{formula}
-       <! ⌜$(ts1) =* $(ts2)⌝ ∧ ⌜$(ts1') =* $(ts2')⌝ !>.
-  Proof with auto.
-    generalize dependent ts2.
-    induction ts1 as [|t1 ts1 IH]; simpl; intros; assert (Hl:=H0).
-    - apply of_same_length_nil_inv_l in Hl as ->. simpl. rewrite f_eqlist_nil.
-      f_simpl. f_equiv. apply OfSameLength_pi.
-    - apply of_same_length_cons_inv_l in Hl as (t2&ts2''&->&?). rename ts2'' into ts2.
-      simpl. repeat rewrite f_eqlist_cons. rewrite <- f_and_assoc. f_simpl.
-      rewrite IH... Unshelve.
-      + simpl in H. apply of_same_length_rest in H...
-      + apply of_same_length_rest in H0...
-  Qed.
-
-  Lemma f_eqlist_replace_l ts1 ts1' ts2 {H : OfSameLength ts1 ts2} (Heq : ts1 = ts1') :
-    @FEqList _ ts1 ts2 H ≡@{formula} @FEqList _ ts1' ts2 (of_same_length_eq_l H Heq).
-  Proof. subst. f_equiv. apply OfSameLength_pi. Qed.
-
-  Lemma f_eqlist_replace_r ts1 ts2 ts2' {H : OfSameLength ts1 ts2} (Heq : ts2 = ts2') :
-    @FEqList _ ts1 ts2 H ≡@{formula} @FEqList _ ts1 ts2' (of_same_length_eq_r H Heq).
-  Proof. subst. f_equiv. apply OfSameLength_pi. Qed.
-
-  Lemma f_eqlist_replace {ts1 ts1' ts2 ts2'} {H : OfSameLength ts1 ts2} :
-    ∀ Heq1 : ts1 = ts1',
-    ∀ Heq2 : ts2 = ts2',
-    @FEqList _ ts1 ts2 H ≡@{formula} @FEqList _ ts1' ts2' (of_same_length_eq H Heq1 Heq2).
-  Proof. intros. subst. f_equiv. apply OfSameLength_pi. Qed.
 
 (* Ltac split_eqlist_fmap_app l1 l2 f g := *)
 (*   repeat match goal with *)
@@ -436,79 +63,67 @@ Section refinement.
 (*         idtac f l1 *)
 (*     end. *)
 
+(* Notation "↑ₓ xs" := (as_var <$> xs : list variable) (at level 0, *)
+(*                       xs constr at level 0) : refiney_scope. *)
+(* Notation "↑₀ xs" := (initial_var_of <$> xs : list variable) (at level 0, *)
+(*                       xs constr at level 0) : refiney_scope. *)
+(* Notation "⇑ₓ xs" := (TVar ∘ as_var <$> xs : list term) (at level 0, *)
+(*                       xs constr at level 0) : refiney_scope. *)
+(* Notation "⇑₀ xs" := (TVar ∘ initial_var_of <$> xs : list term) (at level 0, *)
+(*                       xs constr at level 0) : refiney_scope. *)
+(* Notation "⇑ₜ ts" := (as_term <$> ts : list term) (at level 0, *)
+(*                       ts constr at level 0) : refiney_scope. *)
+(* Notation "₀ xs" := (initial_var_of <$> xs : list variable) (at level 0, *)
+(*                       xs constr at level 0) : refiney_scope. *)
 
-Notation "' xs" := (TVar ∘ as_var <$> xs : list term)
-                       (in custom term at level 0,
-                           xs constr at level 0) : refiney_scope.
-Notation "'₀ xs" := (TVar ∘ initial_var_of <$> xs : list term)
-                       (in custom term at level 0,
-                           xs constr at level 0) : refiney_scope.
-  Lemma subst_initials_seqsubst_lists_unique xs :
-    @seqsubst_lists_unique M (initial_var_of <$> xs) (TVar ∘ as_var <$> xs).
-  Proof.
-    unfold seqsubst_lists_unique. intros.
-    rewrite elem_of_list_pair_indexed in H0, H1. destruct H0 as []. destruct H1 as [].
-    apply list_lookup_fmap_inv in H0 as (x1&?&?).
-    apply list_lookup_fmap_inv in H1 as (x2&?&?).
-    apply list_lookup_fmap_inv in H2 as (x3&?&?).
-    apply list_lookup_fmap_inv in H3 as (x4&?&?).
-    rewrite H4 in H6. inversion H6. subst x3. rewrite H5 in H7.
-    inversion H7. subst x4. clear H6 H7. rewrite H0 in H1.
-    rewrite H2. rewrite H3. f_equal. apply initial_var_of_inj in H1. assumption.
-  Qed.
+(* Notation "xs |ₓ" := (as_var <$> xs : list variable) (at level 0). *)
+(* Notation "xs |ₓ₀" := (initial_var_of <$> xs : list variable) (at level 0). *)
+(* Notation "xs |ₜ" := (TVar ∘ as_var <$> xs : list term) (at level 0). *)
+(* Axiom xs : list final_variable. *)
+(* Definition x := xs|ₓ₀. *)
+(* Definition t := xs|ₜ. *)
+(* Notation "'ₓ( xs )" := (as_var <$> xs : list term) (at level 0). *)
+(* Notation "' xs" := (TVar ∘ as_var <$> xs : list term) *)
+(*                        (in custom term at level 0, *)
+(*                            xs constr at level 0) : refiney_scope. *)
+(* Notation "'₀ xs" := (TVar ∘ initial_var_of <$> xs : list term) *)
+(*                        (in custom term at level 0, *)
+(*                            xs constr at level 0) : refiney_scope. *)
 
-  Lemma subst_initials_vars_terms_disjoin xs :
-    list_to_set (initial_var_of <$> xs) ## ⋃ (@term_fvars value <$> (TVar ∘ as_var <$> xs)).
-  Proof.
-    (* Set Printing Coercions. Unset Printing Notations. *)
-    intros x0 H1 H2. set_unfold. destruct H1 as (x&?&?). subst.
-    apply elem_of_union_list in H2 as (fvars&?&?).
-    apply elem_of_list_fmap in H as (x1&?&?). apply elem_of_list_fmap in H2 as (x2&?&?).
-    subst x1. simpl in H. subst fvars. apply elem_of_singleton in H1.
-    apply initial_var_of_eq_final_variable in H1 as [].
-  Qed.
+(* Notation "%% t" := (as_term t) *)
+(*                      (in custom term at level 0, only parsing, *)
+(*                          t constr at level 0) : refiney_scope. *)
+(* (* Notation "% x" := (as_var x) *) *)
+(* (*                        (in custom term at level 0, *) *)
+(* (*                            only parsing, *) *)
+(* (*                            x constr at level 0) : refiney_scope. *) *)
+(* Notation "% xs" := (as_var <$> xs) *)
+(*                        (in custom term at level 0, *)
+(*                            xs constr at level 0) : refiney_scope. *)
 
-  Hint Resolve subst_initials_seqsubst_lists_unique : core.
-  Hint Resolve subst_initials_vars_terms_disjoin : core.
+(* Notation "%₀ xs" := (initial_var_of <$> xs) *)
+(*                        (in custom term at level 0, *)
+(*                            xs constr at level 0) : refiney_scope. *)
 
-  Lemma fold_subst_initials A w :
-    seqsubst A (initial_var_of <$> w) (TVar ∘ as_var <$> w) = <! A[_₀\ w] !>.
-  Proof. reflexivity. Qed.
+(* Notation "% A" := (as_formula A) *)
+(*                     (in custom formula at level 0, only parsing, *)
+(*                         A constr at level 0) : refiney_scope. *)
 
-  Lemma seqsubst_non_free A (xs : list variable) ts `{OfSameLength _ _ xs ts} :
-    formula_fvars A ## list_to_set xs →
-    <! A[; *xs \ *ts ;] !> ≡ A.
-  Proof with auto.
-    generalize dependent ts. induction xs as [|x xs IH]; intros; assert (Hl:=H).
-    - apply of_same_length_nil_inv_l in Hl as ->. simpl...
-    - apply of_same_length_cons_inv_l in Hl as (t&ts'&->&?). rename ts' into ts. simpl...
-      rewrite IH.
-      2:{ set_solver. }
-      rewrite fequiv_subst_non_free... set_solver.
-  Qed.
-
-  Lemma f_drop_subst_initials A w :
-    formula_final A →
-    <! A[_₀\ w] !> ≡ A.
-  Proof.
-    intros. unfold subst_initials. apply seqsubst_non_free. intros x0 ? ?.
-    set_unfold. destruct H1 as (x&?&?). apply H in H0. unfold var_final in H0.
-    rewrite H1 in H0. simpl in H0. discriminate.
-  Qed.
-
+(* Notation "↑ₓ x" := () *)
+(* ₜₓ *)
 
   Lemma r_assignment w xs pre post ts `{FormulaFinal _ pre} `{OfSameLength _ _ xs ts} :
     length xs ≠ 0 →
     NoDup xs →
-    <! ⌜'₀w =* 'w⌝ ∧ ⌜'₀xs =* 'xs⌝ ∧ pre !> ⇛ <! post[[ *$(as_var <$> xs) \ *$(as_term <$> ts) ]] !> ->
+    <! ⎡⇑₀ w =* ⇑ₓ w⎤ ∧ ⎡⇑₀ xs =* ⇑ₓ xs⎤ ∧ pre !> ⇛ <! post[[ ↑ₓ xs \ ⇑ₜ ts ]] !> ->
     <{ *w, *xs : [pre, post] }> ⊑ <{ *xs := *$(FinalRhsTerm <$> ts)  }>.
   Proof with auto.
     intros Hlength Hnodup proviso A Hfinal. simpl. rewrite wp_asgn.
     assert (<! pre !> ≡ <! pre [_₀\w ++ xs] !>) as ->.
-    { rewrite f_drop_subst_initials... }
+    { rewrite f_subst_initials_final_formula...  }
     rewrite <- simpl_subst_initials_and. rewrite fmap_app.
     unfold subst_initials. rewrite <- f_foralllist_one_point...
-    rewrite f_foralllist_app. rewrite (f_foralllist_drop_binders (as_var <$> w)).
+    rewrite f_foralllist_app. rewrite (f_foralllist_elim_binders (as_var <$> w)).
     rewrite (f_foralllist_elim_as_ssubst <! post ⇒ A !> _ (as_term <$> ts))...
     2:{ rewrite length_fmap... }
     2:{ apply NoDup_fmap... apply as_var_inj. }
@@ -523,7 +138,7 @@ Notation "'₀ xs" := (TVar ∘ initial_var_of <$> xs : list term)
     3: { rewrite <- fmap_app. reflexivity. }
     pose proof (@f_foralllist_one_point M
                   (initial_var_of <$> (w ++ xs)) ((TVar ∘ as_var <$> (w++xs)))) as ->...
-    rewrite fold_subst_initials. rewrite f_drop_subst_initials.
+    rewrite fold_subst_initials. rewrite f_subst_initials_final_formula.
     2: { unfold formula_final. intros. apply fvars_ssubst_superset in H1.
          set_unfold. destruct H1.
          - apply Hfinal...
@@ -535,105 +150,6 @@ Notation "'₀ xs" := (TVar ∘ initial_var_of <$> xs : list term)
     reflexivity.
   Qed.
 
-    rewrite H1... rewrite simult_subst_
-    2: {  }
-
-    Set Printing Coercions.
-    rewrite f_foralllist_one_point.
-    4: { do 2 rewrite fmap_app. do 2 rewrite <- list_fmap_compose. reflexivity. }
-    3: { rewrite fmap_app. reflexivity. }
-    2:{ rewrite length_fmap... }
-    2:{ apply NoDup_fmap... apply as_var_inj. }
-    erewrite f_eqlist_replace. Unshelve.
-    rewrite f_foralllist_impl_unused_r.
-    rewrite f_impl_elim.
-    f_impl_elim
-    rewrite <- f_and_assoc at 2.
-    rewrite proviso.
-    Unshelve.
-    pose proof (fmap_app ((@TVar value) ∘ as_var) w xs).
-    assert (OfSameLength (initial_var_of <$> w ++ xs) ((@TVar value) ∘ as_var <$> w ++ xs) =
- OfSameLength (initial_var_of <$> w ++ xs) ((TVar ∘ as_var <$> w) ++ ((@TVar value) ∘ as_var <$> xs))).
-    { rewrite H1. reflexivity. }
-    Unset Printing Notations. Set Printing Implicit.
-    rewrite simpl_ssubst_impl.
-    split_eqlist_fmap_app w xs (initial_var_of) ((@TVar (value)) ∘ as_var).
-
-    clear.
-    pose proof (f_eqlist_fmap_app w xs (initial_var_of) (TVar ∘ as_var)).
-    unfold fmap.
-    rewrite H1.
-
-    assert (<! ⌜@*(initial_var_of <$> w ++ xs) =* $(fmap (TVar ∘ as_var) (w ++ xs))⌝
-              ⇒ pre ∧ (∀* $(fmap as_var (w ++ xs)),  post ⇒ A) !> ⇛
-            <! ⌜@*(initial_var_of <$> w ++ xs) =* $(fmap (TVar ∘ as_var) (w ++ xs))⌝
-            ⇒ post[[ *$(as_var <$> xs) \ *$(as_term <$> ts)]]
-              ∧ (∀* $(fmap as_var (w ++ xs)),  post ⇒ A) !> ).
-    { admit. }
-    rewrite H1. clear H1.
-
-
-
-    assert
-      (<! ⌜₀x = x⌝ ⇒ (pre ∧ (∀ x, post ⇒ A)) !> ⇛
-                                <! ⌜₀x = x⌝ ⇒ (post [x \ t] ∧ (∀ x, post ⇒ A)) !>).
-    { intros σ ?. rewrite simpl_feval_fimpl in H0. rewrite simpl_feval_fimpl. intros.
-      simp feval in *. apply H0 in H1 as H2. destruct H2 as []. split... apply H.
-      simp feval. split... }
-
-    rewrite fmap_app.
-
-         as_var_ne
-
-        2: {
-        injection H4.
-        initial_var_of
-        Unset Printing Notations.
-        rewrite H3 in H4. inversion H4.
-        rewrite H7 in H9. inversion H9.
-
-        naive_solver.
-        rewrite elem_of_list_pair_indexed in H3.
-    remember ((<! pre ∧ $(FForallList (as_var <$> w ++ xs ++ []) <! post ⇒ A !>) !>)) as C.
-    set ( initial_var_of <$> w ++ xs) as X.
-    set ( (@TVar value) ∘ as_var <$> w ++ xs) as Y.
-    (* pose proof (@f_foralllist_one_point _ X Y C). *)
-    pose proof (@f_foralllist_one_point M).
-    (* subst X. subst Y. *)
-    Unset Printing Notations.
-    Set Printing Implicit.
-
-    rewrite <- f_foralllist_one_point with (xs:=X) (ts:=Y) (A:=C).
-    rewrite <- f_foralllist_one_point.
-    intros H A Hfree. simpl.
-    assert (<! pre !> ≡ <! pre [_₀\list_to_set (w ++ xs)] !>).
-    { unfold subst_initials. admit. }
-    rewrite H1. simpl.
-    simpl. f_simpl.
-    (* intros pre post x t H A Hfree. simpl. *)
-    (* assert (<! %pre !> ≡ pre [₀ x \ x]). *)
-    (* { rewrite fequiv_subst_non_free... pose proof (final_formula_final pre). *)
-    (*   destruct (decide (₀x ∈ formula_fvars pre))... apply H0 in e. simpl in e. discriminate. } *)
-    rewrite H0. clear H0.
-    rewrite <- simpl_subst_and.
-    rewrite <- (f_forall_one_point).
-    2:{ simpl. rewrite not_elem_of_singleton. apply initial_var_of_ne. }
-    assert
-      (<! ⌜₀x = x⌝ ⇒ (pre ∧ (∀ x, post ⇒ A)) !> ⇛
-                                <! ⌜₀x = x⌝ ⇒ (post [x \ t] ∧ (∀ x, post ⇒ A)) !>).
-    { intros σ ?. rewrite simpl_feval_fimpl in H0. rewrite simpl_feval_fimpl. intros.
-      simp feval in *. apply H0 in H1 as H2. destruct H2 as []. split... apply H.
-      simp feval. split... }
-    rewrite H0. clear H0. rewrite (f_forall_elim t x). rewrite simpl_subst_impl.
-    f_simpl. rewrite f_forall_one_point.
-    2:{ simpl. rewrite not_elem_of_singleton. apply initial_var_of_ne. }
-    rewrite fequiv_subst_non_free.
-    2:{ destruct (decide (₀x ∈ formula_fvars <! A [x \ t] !>))... exfalso.
-        apply fvars_subst_superset in e. apply elem_of_union in e. destruct e.
-        - apply Hfree in H0. simpl in H0. discriminate.
-        - pose proof (final_term_final t). apply H1 in H0. simpl in H0. discriminate. }
-    reflexivity.
-  Qed.
 
   Lemma r_alternation
 
