src/Stdppp.v
@@ -76,6 +76,9 @@ Proof with auto.
   intros. unfold lookup_total, map_lookup_total. rewrite lookup_union_r...
 Qed.
 
+
+
+(** Facts about [list] *)
 Lemma length_nonzero_iff_cons {A} (l : list A) n :
   length l = S n ↔ ∃ x xs, l = x :: xs ∧ length xs = n.
 Proof with auto.
@@ -84,10 +87,22 @@ Proof with auto.
   - destruct H as (?&?&->&?). simpl. lia.
 Qed.
 
+Lemma list_lookup_None {A} (l : list A) i :
+  l !! i = None ↔ length l ≤ i.
+Proof with auto.
+  generalize dependent i. induction l; intros.
+  - rewrite lookup_nil. simpl. split... lia.
+  - rewrite lookup_cons. destruct i.
+    + simpl. split; intros; [discriminate | lia].
+    + simpl. rewrite IHl. split; lia.
+Qed.
 
 
-
-
+(** [OfSameLength] type class provides a compositional way to limit pairs of lists
+    to those of the same length. It uses the power of instance synthesization to
+    deduce length equality of lists based on syntatic structure of lists.
+    The main use case for this is in zip pairs. We can prove more intersting facts
+    about the zipped result of two lists, if we know they are of the same length. *)
 Class OfSameLength {A B} (l1 : list A) (l2 : list B) :=
   of_same_length : length l1 = length l2.
 
@@ -128,6 +143,23 @@ Proof. unfold OfSameLength in *. do 2 rewrite length_fmap. assumption. Qed.
 Definition of_same_length_rest {A B} {x1 : A} {l1 : list A} {x2 : B} {l2 : list B}
                               (H : OfSameLength (x1::l1) (x2::l2)) : OfSameLength l1 l2.
 Proof. unfold OfSameLength in *. simpl in H. lia. Defined.
+
+Definition of_same_length_eq_l {A B} {l1 l1' : list A} {l2 : list B} (H : OfSameLength l1 l2) :
+  l1 = l1' →
+  OfSameLength l1' l2.
+Proof. intros. subst. exact H. Qed.
+
+Definition of_same_length_eq_r {A B} {l1 : list A} {l2 l2' : list B} (H : OfSameLength l1 l2) :
+  l2 = l2' →
+  OfSameLength l1 l2'.
+Proof. intros. subst. exact H. Qed.
+
+Definition of_same_length_eq {A B} {l1 l1' : list A} {l2 l2' : list B} (H : OfSameLength l1 l2) :
+  l1 = l1' →
+  l2 = l2' →
+  OfSameLength l1' l2'.
+Proof. intros. subst. exact H. Qed.
+
 
 Instance of_same_length_rev {A B} {l1 : list A} {l2 : list B}
                               `{OfSameLength _ _ l1 l2} : OfSameLength (rev l1) (rev l2).
@@ -174,11 +206,22 @@ Proof.
   apply length_nonzero_iff_cons in H. exact H.
 Qed.
 
-
-
-
-
-
+Lemma elem_of_zip_with_indexed {A B C} (c : C) (xs : list A) (ys : list B) (f : A → B → C)
+    `{OfSameLength _ _ xs ys} :
+  c ∈ zip_with f xs ys ↔ ∃ i x y, xs !! i = Some x ∧ ys !! i = Some y ∧ c = f x y.
+Proof with auto.
+  split; intros.
+  - generalize dependent ys. induction xs as [| x xs IH]; simpl; intros.
+    + apply of_same_length_nil_inv_l in H as ->. apply elem_of_nil in H0 as [].
+    + assert (Hl:=H). apply of_same_length_cons_inv_l in H as (y&ys'&->&?).
+      rename ys' into ys. apply of_same_length_rest in Hl. apply elem_of_cons in H0 as [].
+      * exists 0, x, y. split_and!...
+      * apply (IH _ Hl) in H0 as (i&x'&y'&?&?&?). exists (S i), x', y'. simpl.
+        split_and!...
+  - destruct H0 as (i&x&y&?&?&?). apply elem_of_list_split_length in H0 as (xs0&xs1&->&?).
+    apply elem_of_list_split_length in H1 as (ys0&ys1&->&?). subst i. rewrite zip_with_app...
+    apply elem_of_app. right. simpl. apply elem_of_cons. left...
+Qed.
 
 Lemma dom_list_to_map_zip_L {K A} `{Countable K} (ks : list K) (xs : list A)
     `{OfSameLength K A ks xs} :
@@ -232,6 +275,67 @@ Definition universal_relation {A} (_ _ : A) := True.
 
 Instance universal_relation_equivalence {A} : Equivalence (@universal_relation A).
 Proof. split; hnf; naive_solver. Qed.
+
+#[global] Hint Unfold universal_relation : core.
+
+(** Zip pairs: A zip pair is a pair of two lists that are zipped together.
+    In this section we define two notions of membership for zip pairs and
+    prove some properties about them. *)
+Instance zip_pair_elem_of_with_index {A B} : ElemOf (nat * (A * B)) (list A * list B) :=
+  λ p1 p2, p2.1 !! p1.1 = Some p1.2.1 ∧ p2.2 !! p1.1 = Some p1.2.2.
+
+Instance zip_pair_elem_of {A} {B} : ElemOf (A * B) (list A * list B) :=
+  λ p1 p2, ∃ i, (i, p1) ∈ p2.
+
+Lemma elem_of_zip_pair {A B} (x : A) (y : B) (xs : list A) (ys : list B) :
+  (x, y) ∈ (xs, ys) ↔ ∃ i, xs !! i = Some x ∧ ys !! i = Some y.
+Proof. reflexivity. Qed.
+
+Lemma not_elem_of_zip_pair_inv {A B} (x : A) (y : B) (xs : list A) (ys : list B) :
+  (x, y) ∉ (xs, ys) → ¬ ∃ i, xs !! i = Some x ∧ ys !! i = Some y.
+Proof. rewrite elem_of_zip_pair. auto. Qed.
+
+Lemma not_elem_of_zip_pair {A B} (x : A) (y : B) (xs : list A) (ys : list B) :
+  (∀ i, xs !! i ≠ Some x ∨ ys !! i ≠ Some y) → (x, y) ∉ (xs, ys).
+Proof.
+  intros. intros contra. apply elem_of_zip_pair in contra as (i&?&?).
+  destruct (H i) as []; contradiction.
+Qed.
+
+Lemma elem_of_zip_pair_indexed {A B} (i : nat) (x : A) (y : B) (xs : list A) (ys : list B) :
+  (i, (x, y)) ∈ (xs, ys) ↔ xs !! i = Some x ∧ ys !! i = Some y.
+Proof. reflexivity. Qed.
+
+
+Lemma elem_of_zip_pair_hd_indexed {A B} x0 y0 x y (xs : list A) (ys : list B) :
+  (0, (x0, y0)) ∈ (x :: xs, y :: ys) ↔ (x0 = x ∧ y0 = y).
+Proof. rewrite elem_of_zip_pair_indexed. simpl. split; naive_solver. Qed.
+
+Lemma elem_of_zip_pair_tl_indexed {A B} i x0 y0 x y (xs : list A) (ys : list B) :
+  (S i, (x0, y0)) ∈ (x :: xs, y :: ys) ↔ (i, (x0, y0)) ∈ (xs, ys).
+Proof.
+  do 2 rewrite elem_of_zip_pair_indexed. simpl. naive_solver.
+Qed.
+
+Definition zip_pair_functional {A B} (xs : list A) (ys : list B) :=
+  ∀ i j x y1 y2, i ≠ j → (i, (x, y1)) ∈ (xs, ys) → (j, (x, y2)) ∈ (xs, ys) → y1 = y2.
+
+Lemma NoDup_zip_pair_functional {A B} (xs : list A) (ys : list B) :
+  NoDup xs →
+  zip_pair_functional xs ys.
+Proof with auto.
+  intros H i j ? ? ? ? ? ?. exfalso. apply H0. rewrite elem_of_zip_pair_indexed in H1.
+  rewrite elem_of_zip_pair_indexed in H2. destruct H1 as [? _]. destruct H2 as [? _].
+  eapply NoDup_lookup with (l:=xs) (x:=x)...
+Qed.
+
+Lemma zip_pair_functional_cons_inv {A B} x y (xs : list A) (ys : list B) :
+  zip_pair_functional (x :: xs) (y :: ys) → zip_pair_functional xs ys.
+Proof with auto.
+  intros. intros i j x0 y1 y2 ? ? ?. unfold zip_pair_functional in H.
+  apply (H (S i) (S j) x0); [lia| |]; apply elem_of_zip_pair_tl_indexed...
+Qed.
+
 
 (* HACK: These are not currently used. I will keep them as reference.
    I should delete them at some point. *)
