src/PredCalc/NAryEquivLemmas.v
@@ -12,85 +12,8 @@ From MRC Require Import PredCalc.SyntacticFacts.
 From MRC Require Import PredCalc.SemanticFacts.
 From MRC Require Import PredCalc.EquivLemmas.
 From MRC Require Import PredCalc.NAry.
-
-(* TODO: move them *)
-Notation "(¬)ₗ" := FNot (only parsing) : refiney_scope.
-Notation "(∧)ₗ" := FAnd (only parsing) : refiney_scope.
-Notation "( X ∧.)ₗ" := (FAnd X) (only parsing) : refiney_scope.
-Notation "(.∧ X )ₗ" := (λ Y, FAnd X Y) (only parsing) : refiney_scope.
-Notation "(∨)ₗ" := FAnd (only parsing) : refiney_scope.
-Notation "( X ∨.)ₗ" := (FOr X) (only parsing) : refiney_scope.
-Notation "(.∨ X )ₗ" := (λ Y, FOr X Y) (only parsing) : refiney_scope.
-Notation "(⇒)ₗ" := FImpl (only parsing) : refiney_scope.
-Notation "( X ⇒.)ₗ" := (FImpl X) (only parsing) : refiney_scope.
-Notation "(.⇒ X )ₗ" := (λ Y, FImpl X Y) (only parsing) : refiney_scope.
-Notation "(⇔)ₗ" := FIff (only parsing) : refiney_scope.
-Notation "( X ⇔.)ₗ" := (FIff X) (only parsing) : refiney_scope.
-Notation "(.⇔ X )ₗ" := (λ Y, FIff X Y) (only parsing) : refiney_scope.
-
-
-
-Instance list_pair_indexed_elem_of {A B} : ElemOf (nat * (A * B)) (list A * list B) :=
-  λ p1 p2, p2.1 !! p1.1 = Some p1.2.1 ∧ p2.2 !! p1.1 = Some p1.2.2.
-
-Instance list_pair_elem_of {A} {B} : ElemOf (A * B) (list A * list B) :=
-  λ p1 p2, ∃ i, (i, p1) ∈ p2.
-
-Lemma elem_of_list_pair {A B} (x : A) (y : B) (xs : list A) (ys : list B) :
-  (x, y) ∈ (xs, ys) ↔ ∃ i, xs !! i = Some x ∧ ys !! i = Some y.
-Proof. reflexivity. Qed.
-
-Lemma not_elem_of_list_pair_inv {A B} (x : A) (y : B) (xs : list A) (ys : list B) :
-  (x, y) ∉ (xs, ys) → ¬ ∃ i, xs !! i = Some x ∧ ys !! i = Some y.
-Proof. rewrite elem_of_list_pair. auto. Qed.
-
-Lemma not_elem_of_list_pair {A B} (x : A) (y : B) (xs : list A) (ys : list B) :
-  (∀ i, xs !! i ≠ Some x ∨ ys !! i ≠ Some y) → (x, y) ∉ (xs, ys).
-Proof.
-  intros. intros contra. apply elem_of_list_pair in contra as (i&?&?).
-  destruct (H i) as []; contradiction.
-Qed.
-
-Lemma elem_of_list_pair_indexed {A B} (i : nat) (x : A) (y : B) (xs : list A) (ys : list B) :
-  (i, (x, y)) ∈ (xs, ys) ↔ xs !! i = Some x ∧ ys !! i = Some y.
-Proof. reflexivity. Qed.
-
-Lemma elem_of_zip_with_same_length {A B C} (c : C) (xs : list A) (ys : list B) (f : A → B → C)
-    `{OfSameLength _ _ xs ys} :
-  c ∈ zip_with f xs ys ↔ ∃ i x y, xs !! i = Some x ∧ ys !! i = Some y ∧ c = f x y.
-Proof with auto.
-  split; intros.
-  - generalize dependent ys. induction xs as [| x xs IH]; simpl; intros.
-    + apply of_same_length_nil_inv_l in H as ->. apply elem_of_nil in H0 as [].
-    + assert (Hl:=H). apply of_same_length_cons_inv_l in H as (y&ys'&->&?).
-      rename ys' into ys. apply of_same_length_rest in Hl. apply elem_of_cons in H0 as [].
-      * exists 0, x, y. split_and!...
-      * apply (IH _ Hl) in H0 as (i&x'&y'&?&?&?). exists (S i), x', y'. simpl.
-        split_and!...
-  - destruct H0 as (i&x&y&?&?&?). apply elem_of_list_split_length in H0 as (xs0&xs1&->&?).
-    apply elem_of_list_split_length in H1 as (ys0&ys1&->&?). subst i. rewrite zip_with_app...
-    apply elem_of_app. right. simpl. apply elem_of_cons. left...
-Qed.
-
-Lemma list_lookup_None {A} (l : list A) i :
-  l !! i = None ↔ length l ≤ i.
-Proof with auto.
-  generalize dependent i. induction l; intros.
-  - rewrite lookup_nil. simpl. split... lia.
-  - rewrite lookup_cons. destruct i.
-    + simpl. split; intros; [discriminate | lia].
-    + simpl. rewrite IHl. split; lia.
-Qed.
-
-Lemma elem_of_list_pair_indexed_hd {A B} x0 y0 x y (xs : list A) (ys : list B) :
-  (0, (x0, y0)) ∈ (x :: xs, y :: ys) ↔ (x0 = x ∧ y0 = y).
-Proof. rewrite elem_of_list_pair_indexed. simpl. split; naive_solver. Qed.
-
-Lemma elem_of_list_pair_indexed_tl {A B} i x0 y0 x y (xs : list A) (ys : list B) :
-  (S i, (x0, y0)) ∈ (x :: xs, y :: ys) ↔ (i, (x0, y0)) ∈ (xs, ys).
-Proof.
-  do 2 rewrite elem_of_list_pair_indexed. simpl. naive_solver.
-Qed.
+From MRC Require Import PredCalc.SimultSubst.
+From MRC Require Import PredCalc.FinalElements.
 
 Section n_ary_lemmas.
   Context {M : model}.
@@ -108,18 +31,6 @@ Section n_ary_lemmas.
   Implicit Types ts : list term.
   Implicit Types Bs Cs Ds : list formula.
   Implicit Types vs : list value.
-
-  (* TODO: can this be equality instead of equivalence *)
-  Lemma f_eqlist_nil `{OfSameLength _ _ [] [] } :
-    <! ⌜[] =* []⌝ !> ≡@{formula} <! true !>.
-  Proof. unfold FEqList. reflexivity. Qed.
-
-  (* TODO: can this be equality instead of equivalence *)
-  Lemma f_eqlist_cons t1 t2 ts1 ts2
-    {H1 : OfSameLength ts1 ts2}
-    {H2 : OfSameLength (t1 :: ts1) (t2 :: ts2)} :
-    <! ⌜$(t1 :: ts1) =* $(t2 :: ts2)⌝ !> ≡ <! ⌜t1 = t2⌝ ∧ ⌜ts1 =* ts2⌝ !>.
-  Proof. unfold FEqList. simpl. reflexivity. Qed.
 
   Lemma f_andlist_elim_andlist' Bs' Bs :
     Bs' ⊆+ Bs →
@@ -477,19 +388,19 @@ Section n_ary_lemmas.
 
   Lemma f_eqlist_redundant_l t1 t2 ts1 ts2 `{OfSameLength _ _ ts1 ts2} :
     (t1, t2) ∈ (ts1, ts2) →
-    <! ⌜t1 = t2⌝ ∧ ⌜ts1 =* ts2⌝ !> ≡ <! ⌜ts1 =* ts2⌝ !>.
+    <! ⌜t1 = t2⌝ ∧ ⎡ts1 =* ts2⎤ !> ≡ <! ⎡ts1 =* ts2⎤ !>.
   Proof with auto.
-    intros. apply elem_of_list_pair in H0 as (i&?&?). unfold FEqList.
-    rewrite f_and_andlist_redundant_l'... apply elem_of_zip_with_same_length...
+    intros. apply elem_of_zip_pair in H0 as (i&?&?). unfold FEqList.
+    rewrite f_and_andlist_redundant_l'... apply elem_of_zip_with_indexed...
     exists i, t1, t2. split_and!...
   Qed.
 
   Lemma f_eqlist_redundant_r t1 t2 ts1 ts2 `{OfSameLength _ _ ts1 ts2} :
     (t1, t2) ∈ (ts1, ts2) →
-    <! ⌜ts1 =* ts2⌝ ∧  ⌜t1 = t2⌝ !> ≡ <! ⌜ts1 =* ts2⌝ !>.
+    <! ⎡ts1 =* ts2⎤ ∧  ⌜t1 = t2⌝ !> ≡ <! ⎡ts1 =* ts2⎤ !>.
   Proof with auto.
-    intros. apply elem_of_list_pair in H0 as (i&?&?). unfold FEqList.
-    rewrite f_and_andlist_redundant_r'... apply elem_of_zip_with_same_length...
+    intros. apply elem_of_zip_pair in H0 as (i&?&?). unfold FEqList.
+    rewrite f_and_andlist_redundant_r'... apply elem_of_zip_with_indexed...
     exists i, t1, t2. split_and!...
   Qed.
 
@@ -700,6 +611,14 @@ Section n_ary_lemmas.
     - intros σ. unfold FForall. rewrite IH... rewrite f_not_stable...
   Qed.
 
+  Lemma f_existslist_as_foralllist xs A :
+    <! ∃* xs, A !> ≡ <! ¬ ∀* xs, ¬ A !>.
+  Proof with auto.
+    induction xs as [|x xs IH]; simpl...
+    - rewrite f_not_stable...
+    - intros σ. unfold FForall. rewrite IH... rewrite f_not_stable...
+  Qed.
+
   (* A.76 *)
   (* TODO: replace all [_ ∩ _ = ∅]s with [_ ## _]s *)
   Lemma f_foralllist_and_unused_l xs A B :
@@ -811,25 +730,6 @@ Section n_ary_lemmas.
 
 
   (* TODO: Move these somewhere *)
-  Definition seqsubst_lists_unique xs ts :=
-    ∀ i j x t1 t2, i ≠ j → (i, (x, t1)) ∈ (xs, ts) → (j, (x, t2)) ∈ (xs, ts) → t1 = t2.
-
-  Lemma NoDup_seqsubst_lists_unique xs ts :
-    NoDup xs →
-    seqsubst_lists_unique xs ts.
-  Proof with auto.
-    intros H i j ? ? ? ? ? ?. exfalso. apply H0. rewrite elem_of_list_pair_indexed in H1.
-    rewrite elem_of_list_pair_indexed in H2. destruct H1 as [? _]. destruct H2 as [? _].
-    eapply NoDup_lookup with (l:=xs) (x:=x)...
-  Qed.
-
-  Lemma seqsubst_lists_unique_cons_inv x t xs ts :
-    seqsubst_lists_unique (x :: xs) (t :: ts) → seqsubst_lists_unique xs ts.
-  Proof with auto.
-    intros. intros i j x0 t1 t2 ? ? ?. unfold seqsubst_lists_unique in H.
-    apply (H (S i) (S j) x0); [lia| |]; apply elem_of_list_pair_indexed_tl...
-  Qed.
-
   (* Lemma fequiv_subst_non_free A x t : *)
   (*   x ∉ formula_fvars A → *)
   (*   <! A[x \ t] !> ≡ A. *)
@@ -932,21 +832,21 @@ Section n_ary_lemmas.
 
   (* A.56 *)
   Lemma f_existslist_one_point xs ts A `{OfSameLength _ _ xs ts} :
-    seqsubst_lists_unique xs ts →
+    zip_pair_functional xs ts →
     (list_to_set xs) ## ⋃ (term_fvars <$> ts) →
-    <! ∃* xs, ⌜@*xs =* ts⌝ ∧ A !> ≡ <! A[; *xs \ *ts ;] !>.
+    <! ∃* xs, ⎡⇑ₓ₊ xs =* ts⎤ ∧ A !> ≡ <! A[; *xs \ *ts ;] !>.
   Proof with auto.
     intros Hunique Hfree. generalize dependent ts.
     induction xs as [|x xs IH]; simpl in *; intros.
     - inversion H. assert (H':=H). apply of_same_length_nil_inv_l in H' as ->.
       simpl. unfold FEqList. simpl. rewrite f_and_comm. apply f_and_true.
     - inversion H. assert (H':=H). apply of_same_length_cons_inv_l in H' as (t&ts'&?&?).
-      subst ts. rename ts' into ts. simpl. rewrite f_eqlist_cons.
-      apply seqsubst_lists_unique_cons_inv in Hunique as Hunique'.
+      subst ts. rename ts' into ts. erewrite eqlist_cons.
+      apply zip_pair_functional_cons_inv in Hunique as Hunique'.
       destruct (decide (x ∈ xs)).
       + assert (e':=e). apply elem_of_list_lookup_1 in e' as [i Hi].
         rewrite f_eqlist_redundant_l.
-        2:{ apply elem_of_list_pair. exists i. split...
+        2:{ apply elem_of_zip_pair. exists i. split...
             - apply list_lookup_fmap_Some. exists x...
             - assert (∃ t', ts !! i = Some t') as (t'&?).
               { apply elem_of_list_split_length in Hi as (xs0&xs1&->&?).
@@ -958,9 +858,8 @@ Section n_ary_lemmas.
               enough (t = t') by (subst t'; apply H0).
               apply Hunique.
               + lia.
-              + apply elem_of_list_pair_indexed_hd. split...
-              + apply elem_of_list_pair_indexed_tl. apply elem_of_list_pair_indexed.
-                split... }
+              + apply elem_of_zip_pair_hd_indexed. split...
+              + apply elem_of_zip_pair_tl_indexed. apply elem_of_zip_pair_indexed... }
         rewrite f_exists_existslist_idemp... rewrite fequiv_subst_non_free.
         * apply IH; [| set_solver]...
         * intros contra.
@@ -970,9 +869,9 @@ Section n_ary_lemmas.
   Qed.
 
   Lemma f_foralllist_one_point xs ts A `{OfSameLength _ _ xs ts} :
-    seqsubst_lists_unique xs ts →
+    zip_pair_functional xs ts →
     (list_to_set xs) ## ⋃ (term_fvars <$> ts) →
-    <! ∀* xs, ⌜@*xs =* ts⌝ ⇒ A !> ≡ <! A[; *xs \ *ts ;] !>.
+    <! ∀* xs, ⎡⇑ₓ₊ xs =* ts⎤ ⇒ A !> ≡ <! A[; *xs \ *ts ;] !>.
   Proof with auto.
     intros. rewrite f_foralllist_as_existslist. rewrite f_not_impl.
     rewrite f_existslist_one_point... rewrite simpl_seqsubst_not. rewrite f_not_stable...
@@ -1117,6 +1016,62 @@ Section n_ary_lemmas.
   (*   exists v. rewrite (feval_subst v) in H... rewrite (feval_subst v)... *)
   (* Qed. *)
 
+  Lemma f_foralllist_elim_as_ssubst A (xs : list variable) ts `{OfSameLength _ _ xs ts} :
+    length xs ≠ 0 →
+    NoDup xs →
+    <! ∀* xs, A !> ⇛ <! A[[*xs \ *ts]] !>.
+  Proof with auto.
+    generalize dependent ts. generalize dependent A.
+    induction xs as [|x xs IH]; intros; assert (Hl:=H).
+    1: { simpl in H0. contradiction. }
+    apply of_same_length_cons_inv_l in Hl as (t&ts'&->&?). rename ts' into ts.
+    clear H0. destruct (length xs) eqn:E.
+    1:{ apply length_zero_iff_nil in E, H2. subst. simpl in H1. rewrite (ssubst_single A x t).
+        apply f_forall_elim... }
+    apply of_same_length_rest in H as ?. clear E. simpl. assert (Hunique:=H1).
+    apply NoDup_cons in H1 as []. rewrite f_forall_foralllist_comm.
+    intros σ ?. pose proof (teval_total σ t) as [vt Hvt].
+    rewrite f_forall_elim with (t:=TConst vt) in H4.
+    specialize (IH <! A[x \ $(TConst vt)] !> ts H0). forward IH by lia.
+    rewrite IH in H4... rewrite <- ssubst_extract_inside in H4...
+    2: { simpl. set_solver. }
+    pose proof (teval_var_term_map_total σ (to_var_term_map (x::xs) (t::ts))) as (mv&?).
+    rewrite feval_simult_subst with (mv:=mv)...
+    pose proof (teval_var_term_map_total σ (to_var_term_map (x::xs) ((TConst vt)::ts))) as (mv'&?).
+    rewrite feval_simult_subst with (mv:=mv') in H4...
+    enough (mv = mv') by (subst mv'; assumption). clear H2 IH H4 A.
+    apply of_same_length_rest in H as Hl.
+    apply teval_var_term_map_zip_cons_inv with (H:=Hl) in H5 as (v&mv0&?&->&?&?)...
+    apply teval_var_term_map_zip_cons_inv with (H:=Hl) in H6 as (v'&mv1&?&->&?&?)...
+    inversion H6. subst v0. subst v'. pose proof (teval_det t vt v Hvt H2) as ->.
+    pose proof (teval_var_term_map_det _ _ _ H5 H8) as ->...
+  Qed.
+
+  Lemma f_exists_intro_as_ssubst A (xs : list variable) ts `{OfSameLength _ _ xs ts} :
+    length xs ≠ 0 →
+    NoDup xs →
+    <! A[[*xs \ *ts]] !> ⇛ <! ∃* xs, A !>.
+  Proof with auto.
+    intros. rewrite f_existslist_as_foralllist. rewrite <- f_ent_contrapositive.
+    rewrite f_not_stable. rewrite <- simpl_ssubst_not. apply f_foralllist_elim_as_ssubst...
+  Qed.
+
+  Lemma f_foralllist_elim_binders (xs : list variable) A :
+    <! ∀* xs, A !> ⇛ <! A !>.
+  Proof with auto.
+    induction xs as [|x xs IH]; simpl.
+    - reflexivity.
+    - rewrite IH. rewrite f_forall_elim_binder. reflexivity.
+  Qed.
+
+  Lemma f_existslist_intro_binders (xs : list variable) A :
+    <! A !> ⇛ <! ∃* xs, A !>.
+  Proof with auto.
+    rewrite f_existslist_as_foralllist. rewrite <- f_ent_contrapositive. rewrite f_not_stable.
+    apply f_foralllist_elim_binders.
+  Qed.
+
+
   (* Lemma f_impl_elim A B : *)
   (*   <! A ∧ (A ⇒ B) !> ⇛ B. *)
   (* Proof with auto. *)
@@ -1234,4 +1189,60 @@ Section n_ary_lemmas.
   (* Proof. *)
   (*   rewrite f_eq_refl. rewrite f_not_true. reflexivity. *)
   (* Qed. *)
+
+  Lemma f_existslist_app (xs1 xs2 : list variable) A :
+    <! ∃* $(xs1 ++ xs2), A !> ≡ <! ∃* xs1, ∃* xs2, A !>.
+  Proof with auto.
+    induction xs1 as [|x1 xs1 IH]... simpl. rewrite IH...
+  Qed.
+
+  Lemma f_foralllist_app (xs1 xs2 : list variable) A :
+    <! ∀* $(xs1 ++ xs2), A !> ≡ <! ∀* xs1, ∀* xs2, A !>.
+  Proof with auto.
+    induction xs1 as [|x1 xs1 IH]... simpl. rewrite IH...
+  Qed.
+
+  (** [FEqList] facts *)
+  Lemma f_eqlist_app ts1 ts1' ts2 ts2'
+                          `{OfSameLength _ _ (ts1 ++ ts1') (ts2 ++ ts2')}
+                          `{OfSameLength _ _ ts1 ts2}
+                          `{OfSameLength _ _ ts1' ts2'} :
+    <! ⎡$(ts1 ++ ts1') =* $(ts2 ++ ts2')⎤ !> ≡@{formula}
+       <! ⎡$(ts1) =* $(ts2)⎤ ∧ ⎡$(ts1') =* $(ts2')⎤ !>.
+  Proof with auto.
+    generalize dependent ts2.
+    induction ts1 as [|t1 ts1 IH]; simpl; intros; assert (Hl:=H0).
+    - apply of_same_length_nil_inv_l in Hl as ->. simpl. rewrite eqlist_nil.
+      rewrite f_and_comm. rewrite f_and_true. f_equiv. apply OfSameLength_pi.
+    - apply of_same_length_cons_inv_l in Hl as (t2&ts2''&->&?). rename ts2'' into ts2.
+      simpl. repeat erewrite eqlist_cons. rewrite <- f_and_assoc. apply f_and_cancel_l.
+      rewrite IH... Unshelve.
+      + simpl in H. apply of_same_length_rest in H...
+      + apply of_same_length_rest in H0...
+  Qed.
+
+  Lemma f_eqlist_replace_l ts1 ts1' ts2 {H : OfSameLength ts1 ts2} (Heq : ts1 = ts1') :
+    @FEqList _ ts1 ts2 H ≡@{formula} @FEqList _ ts1' ts2 (of_same_length_eq_l H Heq).
+  Proof. subst. f_equiv. apply OfSameLength_pi. Qed.
+
+  Lemma f_eqlist_replace_r ts1 ts2 ts2' {H : OfSameLength ts1 ts2} (Heq : ts2 = ts2') :
+    @FEqList _ ts1 ts2 H ≡@{formula} @FEqList _ ts1 ts2' (of_same_length_eq_r H Heq).
+  Proof. subst. f_equiv. apply OfSameLength_pi. Qed.
+
+  Lemma f_eqlist_replace {ts1 ts1' ts2 ts2'} {H : OfSameLength ts1 ts2} :
+    ∀ Heq1 : ts1 = ts1',
+    ∀ Heq2 : ts2 = ts2',
+    @FEqList _ ts1 ts2 H ≡@{formula} @FEqList _ ts1' ts2' (of_same_length_eq H Heq1 Heq2).
+  Proof. intros. subst. f_equiv. apply OfSameLength_pi. Qed.
+
+  (** [subst_initials] facts *)
+  Lemma f_subst_initials_final_formula A w :
+    formula_final A →
+    <! A[_₀\ w] !> ≡ A.
+  Proof.
+    intros. unfold subst_initials. apply seqsubst_non_free. intros x0 ? ?.
+    set_unfold. destruct H1 as (x&?&?). apply H in H0. unfold var_final in H0.
+    rewrite H1 in H0. simpl in H0. discriminate.
+  Qed.
+
 End n_ary_lemmas.
