src/SeqNotation.v
@@ -1,47 +1,40 @@
 From Stdlib Require Import Lists.List. Import ListNotations.
+From stdpp Require Import base.
 From MRC Require Import Prelude.
+From MRC Require Import Model.
 
-Declare Custom Entry bracketed_seq_notation.
-Declare Custom Entry seq_notation.
-Declare Custom Entry seq_elem.
+Declare Custom Entry var_seq.
+Declare Custom Entry var_seq_elem.
 
-Notation "⟨ xs ⟩" := (xs) (in custom bracketed_seq_notation, only parsing,
-                           xs custom seq_elem)
+Notation "xs" := (xs) (in custom var_seq at level 0,
+                       xs custom var_seq_elem)
     : refiney_scope.
-Notation "xs" := (xs) (in custom bracketed_seq_notation at level 0,
-                       only printing,
-                       xs custom seq_elem)
-    : refiney_scope.
-Notation "∅" := ([]) (in custom bracketed_seq_notation at level 0)
-    : refiney_scope.
-Notation "* xs" := xs (in custom bracketed_seq_notation at level 0,
-                         xs constr at level 0,
-                         only parsing)
-    : refiney_scope.
-Notation "*$( xs )" := xs (in custom bracketed_seq_notation at level 0,
-                             xs constr at level 200,
-                             only parsing)
+Notation "∅" := ([]) (in custom var_seq at level 0)
     : refiney_scope.
 
-
-
-Notation "xs" := (xs) (in custom seq_notation at level 0,
-                       xs custom seq_elem)
+Notation "x" := ([x]) (in custom var_seq_elem at level 0, x constr at level 0)
     : refiney_scope.
-Notation "∅" := ([]) (in custom seq_notation at level 0)
+Notation "↑ₓ xs" := (as_var <$> xs : list variable)
+                      (in custom var_seq_elem at level 5, xs constr at level 0)
     : refiney_scope.
-
-Notation "x" := ([x]) (in custom seq_elem at level 0, x constr at level 0)
+Notation "↑ₓ( xs )" := (as_var <$> xs : list variable)
+                      (in custom var_seq_elem at level 5, only parsing, xs constr at level 200)
     : refiney_scope.
-Notation "$( x )" := ([x]) (in custom seq_elem at level 5,
+Notation "↑₀ xs" := (initial_var_of <$> xs : list variable)
+                      (in custom var_seq_elem at level 5, xs constr at level 0)
+    : refiney_scope.
+Notation "↑₀( xs )" := (initial_var_of <$> xs : list variable)
+                      (in custom var_seq_elem at level 5, only parsing, xs constr at level 200)
+    : refiney_scope.
+Notation "$( x )" := ([x]) (in custom var_seq_elem at level 5,
                            only parsing,
-                             x constr at level 200)
+                           x constr at level 200)
     : refiney_scope.
-Notation "* x" := x (in custom seq_elem at level 0, x constr at level 0)
+Notation "* x" := x (in custom var_seq_elem at level 0, x constr at level 0)
     : refiney_scope.
-Notation "*$( x )" := x (in custom seq_elem at level 5, x constr at level 200)
+Notation "*$( x )" := x (in custom var_seq_elem at level 5, only parsing, x constr at level 200)
     : refiney_scope.
-Infix "," := app (in custom seq_elem at level 10, right associativity) : refiney_scope.
+Infix "," := app (in custom var_seq_elem at level 10, right associativity) : refiney_scope.
 (* Open Scope refiney_scope. *)
 (* Notation "'seq' s" := s (at level 10, s custom seq_notation). *)
 
